% Set up the document
\documentclass{article}

% Page size
\usepackage[
    letterpaper,]{geometry}

% Lines between paragraphs
\setlength{\parskip}{\baselineskip}
\setlength{\parindent}{0pt}

% Math
\usepackage{mathtools}
\usepackage{amssymb}
\usepackage{amsthm}
\usepackage{commath}

% Number sets
\newcommand{\Z}{\mathbb{Z}}
\newcommand{\Q}{\mathbb{Q}}
\newcommand{\X}{\mathbb{X}}
\newcommand{\C}{\mathcal{C}}
\newcommand{\N}{\mathbb{N}}
\newcommand{\R}{\mathbb{R}}
\newcommand{\V}{\mathbb{V}}

% Links
\usepackage{hyperref}

% Page numbers at top right
\usepackage{fancyhdr}
\pagestyle{fancy}
\fancyhf{}
\fancyhead[R]{\thepage}
\renewcommand\headrulewidth{0pt}

\begin{document}

\textbf{MATH 320 Worksheet 1} \\
\textbf{Matt Wiens \#301294492} \\
\textbf{2020-01-15}

1. Let $X = \R^n$. Verify that the following are metrics on $X$:

(a)
%
\begin{equation*}
    d_1(x, y) = \sum_{i = 1}^n \envert{x_i - y_i}
    .
\end{equation*}

\textit{Solution.}
We need to verify three properties:

Fix any $x, y, z \in X$.

1. Clearly $d_1(x, y) \geq 0$. Also, we have
%
\begin{align*}
    &d_1(x, y) = 0 \\
    &\iff x_i = y_i, \quad \forall i = 1, \ldots, n \\
    &\iff x = y
    .
\end{align*}
%
2. Here we need to verify the symmetry of $d_1$:
%
\begin{align*}
    d_1(x, y) &= \sum_{i = 1}^n \envert{x_i - y_i} \\
              &= \sum_{i = 1}^n \envert{y_i - x_i} \\
              &= d_1(y, x)
    .
\end{align*}
%
3. For this property we will use the triangle inequality of $|\cdot|$:
%
\begin{align*}
    d_1(x, y) + d_1(y, z)
        &= \sum_{i = 1}^n \envert{x_i - y_i} + \sum_{i = 1}^n \envert{y_i - z_i} \\
        &= \sum_{i = 1}^n \del[2]{\envert{x_i - y_i} + \envert{y_i - z_i}} \\
        &\geq \sum_{i = 1}^n \envert{x_i - z_i} \\
        &= d_1(x, z)
    .
\end{align*}

\vspace{3mm}

(b)
%
\begin{equation*}
    d_2(x, y) = \sqrt{\sum_{i = 1}^n {\envert{x_i - y_i}}^2}
    .
\end{equation*}

\textit{Solution.}
Properties 1 and 2 are verified similarly to what was shown in part (a).
Here we will only verify property 3.

Fix any $x, y, z \in X$. Then
%
\begin{align*}
    d_2(x, z)^2
        &= \sum_{i = 1}^n \envert{x_i - z_i}^2 \\
        &= \sum_{i = 1}^n \envert{(x_i - y_i) - (y_i - z_i)}^2 \\
        &= \sum_{i = 1}^n
            \del{
                \envert{x_i - y_i}^2
                - 2 \envert{x_i - y_i} \envert{y_i - z_i}
                + \envert{y_i - z_i}^2
            } \\
        &= \sum_{i = 1}^n \envert{x_i - y_i}^2
           - 2 \sum_{i = 1}^n \envert{x_i - y_i} \envert{y_i - z_i}
           + \sum_{i = 1}^n \envert{y_i - z_i}^2 \\
        &= d_2(x, y)^2
           - 2 \sum_{i = 1}^n \envert{x_i - y_i} \envert{y_i - z_i}
           + d_2(y, z)^2 \\
        &\leq d_2(x, y)^2 + d_2(y, z)^2 \\
        &\leq \del{d_2(x, y) + d_2(y, z)}^2
    .
\end{align*}
%
Taking square roots of both sides of the inequality, we obtain
%
\begin{equation*}
    d_2(x, y) + d_2(y, z) \geq d_2(x, z)
    .
\end{equation*}

\newpage

\end{document}
